\chapter{GHZ}

The GHZ state is defined by

\grayeq{
\beq
\ket{GHZ} =
\frac{1}{\sqrt{2}}
(\ket{000} + \ket{111})
\;.
\eeq}

\claim

\grayeq{
\beq
\ket{GHZ} =
\begin{array}{c}
\Qcircuit @C=1em @R=.5em @!R{
&\timesgate\qwx[2]
&\qw
&\qw
&\gate{\ket{0}}
\\
&\qw
&\timesgate\qwx[1]
&\qw
&\gate{\ket{0}}
\\
&\dotgate
&\dotgate
&\gate{H}
&\gate{\ket{0}}
}
\end{array}
\;.
\label{eq-ghz-ckt}
\eeq}
\proof
Let RHS denote right
hand side of Eq.(\ref{eq-ghz-ckt}).

\beqa
RHS&=&
\cnot{\bitc}{\bita}
\cnot{\bitc}{\bitb}
H(\bitc)
\ket{000}_{\bita\bitb\bitc}
\\
&=&
\cnot{\bitc}{\bita}
\cnot{\bitc}{\bitb}
\frac{1}{\sqrt{2}}\sum_{a\in Bool}\ket{0,0,a}
\\
&=&
\frac{1}{\sqrt{2}}\sum_{a\in Bool}\ket{a,a,a}=\ket{GHZ}
\;.
\eeqa
\qed

\claim

\grayeq{
\beq
\sigma_{XYY}\ket{GHZ}=
\sigma_{YXY}\ket{GHZ}=
\sigma_{YYX}\ket{GHZ}=-\ket{GHZ}
\;.
\label{eq-ghz-xyy}
\eeq}
Hence,

\grayeq{
\beq
\sigma_{XYY}\sigma_{YXY}
\sigma_{YYX}\ket{GHZ}=-\ket{GHZ}
\;.
\label{eq-ghz-3xyy}
\eeq}
However,

\grayeq{
\beq
\sigma_{XXX}\ket{GHZ}=+\ket{GHZ}
\;.
\label{eq-ghz-xxx}
\eeq}
\proof
For any $a\in Bool$,
$\sigy\ket{a}=i(-1)^a\ket{\overline{a}}$ and
$\sigx\ket{a}=\ket{\overline{a}}$ so

\beqa
\sigma_{XYY}\ket{GHZ}&=&
\sigx\otimes\sigy\otimes\sigy
\frac{1}{\sqrt{2}}\sum_{a\in Bool}\ket{a,a,a}
\\
&=&
(-1)\frac{1}{\sqrt{2}}
\sum_a\ket{\overline{a},\overline{a},\overline{a}}\\
&=& -\ket{GHZ}
\;.
\eeqa
This establishes Eq.(\ref{eq-ghz-xyy}).
Eq.(\ref{eq-ghz-3xyy}) follows from
Eq.(\ref{eq-ghz-xyy}).
Eq.(\ref{eq-ghz-xxx}) can be proven in the
same way as Eq.(\ref{eq-ghz-xyy}).
\qed
