\chapter{Hadamard Matrices}

The 1 bit Hadamard matrix is defined by

\beq
H_1 =\frac{1}{\sqrt{2}}
\begin{tabular}{r|rr}
         & {\tiny 0} & {\tiny 1} \\
\hline
{\tiny 0}& 1&  1\\
{\tiny 1}& 1& -1\\
\end{tabular}
\;.
\eeq
The $\nb$-bit Hadamard matrix is defined
as the $\nb$-fold tensor product of $H_1$:

\beq
H_\nb = \underbrace{
H_1\otimes H_1 \otimes \ldots \otimes H_1}_{\mbox{$\nb$ factors}}
\;.
\eeq
For example, for $\nb=2$,

\beq
H_2 =
\frac{1}{2}
\begin{tabular}{r|rrrr}
         & {\tiny 00} & {\tiny 01} & {\tiny 10} & {\tiny 11}\\
\hline
{\tiny 00}&  1&  1&  1&  1\\
{\tiny 01}&  1& -1&  1& -1\\
{\tiny 10}&  1&  1& -1& -1\\
{\tiny 11}&  1& -1& -1&  1\\
\end{tabular}
\;,
\eeq
where we have labelled
the rows and columns with binary numbers
 in increasing dictionary order.
Equivalently, for bits
$\vec{\alpha}=(\alpha_1,
\alpha_1, \ldots, \alpha_{\nb})$,

\beq
H_\nb(\vec{\alpha})=
\prod_{i=1}^{\nb}
H_1(\alpha_i)
\;.
\eeq
We will often use a plain $H$
to represent $H_1$.
Since
$(H_1)_{b,b'} = \frac{(-1)^{bb'}}{\sqrt{2}}$
 for $b, b'\in Bool$,
it follows that

 \beq
 (H_\nb)_{\vec{b},\vec{b'}} =
 \frac{(-1)^{\vec{b}\cdot \vec{b'}}}{\sqrt{2^\nb}}
 \;
 \eeq
 for $\vec{b}, \vec{b'}\in Bool^\nb$ .
Since $H_1^2=1$ and $H_1^T=H_1$, where
T=transpose, it follows that

\beq
H_\nb^2 = 1
\;,
\eeq
and

\beq
H_\nb^T = H_\nb
\;.
\eeq
